src/3d/Options.fsti
@@ -34,6 +34,10 @@ val get_hoist_locals : unit -> ML bool
 
 val get_goto_for_early_return : unit -> ML bool
 
+val get_blank_lines : unit -> ML bool
+
+val get_line_comments : unit -> ML bool
+
 val get_init_locals : unit -> ML (option string)
 
 val get_check_hashes : unit -> ML (option check_hashes_t)
